erasure/theories/Typed/Extraction.v
@@ -43,34 +43,34 @@ Record extract_pcuic_params :=
 
 
 Lemma fresh_global_erase_global_decl_rec :
-    forall (Σ0 : global_declarations) (universes0 : ContextSet.t) (retroknowledge0 : Retroknowledge.t)
-           (wfΣ : ∥ wf ({| PEnv.universes := universes0; PEnv.declarations := Σ0; PEnv.retroknowledge := retroknowledge0 |}) ∥)
+    forall X_type X (Σ0 : global_declarations) (universes0 : ContextSet.t) (retroknowledge0 : Retroknowledge.t)
+           wfΣ
            (seeds : KernameSet.t) (ignore : kername -> bool) kn,
       EnvMap.EnvMap.fresh_global kn Σ0 ->
-      ExAst.fresh_global kn (erase_global_decls_deps_recursive Σ0 universes0 retroknowledge0 wfΣ seeds ignore).
+      ExAst.fresh_global kn (@erase_global_decls_deps_recursive X_type X Σ0 universes0 retroknowledge0 wfΣ seeds ignore).
 Proof.
-  intros Σ0 universes0 retroknowledge0 wfΣ seeds ignore kn fresh.
-  revert wfΣ seeds.
-  induction Σ0;intros wfΣ seeds.
+  intros X_type X Σ0 universes0 retroknowledge0 wfΣ seeds ignore kn fresh.
+  revert X_type X wfΣ seeds.
+  induction Σ0;intros X_type X wfΣ seeds.
   - constructor.
   - cbn. destruct a;cbn.
     inversion fresh;cbn in *;subst;clear fresh.
     destruct (KernameSet.mem _ _) eqn:Hmem;cbn.
     * constructor;auto.
-      now apply IHΣ0.
+      now eapply IHΣ0.
     * now apply IHΣ0.
 Qed.
 
 Lemma fresh_globals_erase_global_decl_rec :
-    forall (Σ0 : global_declarations) (universes0 : ContextSet.t) (retroknowledge0 : Retroknowledge.t)
-           (wfΣ : ∥ wf ({| PEnv.universes := universes0; PEnv.declarations := Σ0; PEnv.retroknowledge := retroknowledge0 |}) ∥)
+    forall X_type X (Σ0 : global_declarations) (universes0 : ContextSet.t) (retroknowledge0 : Retroknowledge.t)
+           wfΣ
            (seeds : KernameSet.t) (ignore : kername -> bool),
       EnvMap.EnvMap.fresh_globals Σ0 ->
-      ExAst.fresh_globals (erase_global_decls_deps_recursive Σ0 universes0 retroknowledge0 wfΣ seeds ignore).
+      ExAst.fresh_globals (@erase_global_decls_deps_recursive X_type X Σ0 universes0 retroknowledge0 wfΣ seeds ignore).
 Proof.
-  intros Σ0 universes0 retroknowledge0 wfΣ seeds ignore fresh.
-  revert wfΣ seeds.
-  induction Σ0;intros wfΣ seeds;cbn in *.
+  intros X_type X Σ0 universes0 retroknowledge0 wfΣ seeds ignore fresh.
+  revert X_type X wfΣ seeds.
+  induction Σ0;intros X_type X wfΣ seeds;cbn in *.
   - constructor.
   - destruct a;cbn.
     inversion fresh;subst.
@@ -87,12 +87,18 @@ Program Definition extract_pcuic_env
            (wfΣ : ∥wf Σ ∥)
            (seeds : KernameSet.t)
            (ignore : kername -> bool) : result ExAst.global_env _ :=
-  let Σ := timed "Erasure" (fun _ => erase_global_decls_deps_recursive (declarations Σ) (universes Σ) (retroknowledge Σ) wfΣ seeds ignore) in
+  let Σ := timed "Erasure"
+    (fun _ => erase_global_decls_deps_recursive (X_type := PCUICWfEnvImpl.optimized_abstract_env_impl (guard := fake_guard_impl_instance))
+      (X := PCUICWfEnvImpl.build_wf_env_from_env Σ wfΣ)
+      (declarations Σ) (universes Σ) (retroknowledge Σ) _ seeds ignore) in
   if optimize_prop_discr params then
     let Σ := timed "Removal of prop discrimination" (fun _ => OptimizePropDiscr.remove_match_on_box_env Σ _) in
     compose_transforms (extract_transforms params) Σ
   else
     Ok Σ.
+Next Obligation.
+  destruct Σ; eauto.
+Qed.
 Next Obligation.
   apply fresh_globals_erase_global_decl_rec.
   sq.
