erasure/theories/Typed/ExtractionCorrectness.v
@@ -1,9 +1,10 @@
-From Coq Require Import List.
+From Coq Require Import List ssreflect ssrbool.
 From MetaCoq.Erasure.Typed Require Import ErasureCorrectness.
 From MetaCoq.Erasure.Typed Require Import ExAst.
 From MetaCoq.Erasure.Typed Require Import Extraction.
 From MetaCoq.Erasure.Typed Require Import Optimize.
 From MetaCoq.Erasure.Typed Require Import OptimizeCorrectness.
+From MetaCoq.Erasure.Typed Require Import OptimizePropDiscr.
 From MetaCoq.Erasure.Typed Require Import ResultMonad.
 From MetaCoq.Erasure.Typed Require Import WcbvEvalAux.
 From Equations Require Import Equations.
@@ -76,21 +77,85 @@ Proof.
 Qed.
 
 Module PEnv := PCUICAst.PCUICEnvironment.
+Import PCUICWfEnv ErasureFunction ErasureFunctionProperties.
 
-(*Lemma wf_erase_global_decl :
-  forall (H : EWellformed.EEnvFlags) (k : kername) (g : PCUICAst.PCUICEnvironment.global_decl)
+Lemma extends_trans Σ Σ' Σ'' :
+  EGlobalEnv.extends Σ Σ' ->
+  EGlobalEnv.extends Σ' Σ'' ->
+  EGlobalEnv.extends Σ Σ''.
+Proof.
+  intros e e' kn h h'.
+  eapply e in h'. now eapply e' in h'.
+Qed.
+
+(* Lemma trans_global_decl_erase {X_type X} :
+  trans_global_decl (@Erasure.erase_global_decl X_type X Σ prf kn decl ond) = *)
+
+Lemma filter_deps_ext deps deps' l :
+  KernameSet.Equal deps deps' ->
+  filter_deps deps l = filter_deps deps' l.
+Proof.
+  induction l as [|[kn d] decls] in deps, deps' |- *; cbn; auto.
+  destruct (KernameSet.mem kn deps) eqn:e.
+  eapply KernameSet.mem_spec in e.
+  intros kne. eapply kne in e. eapply KernameSet.mem_spec in e. rewrite e.
+  rewrite (IHdecls _ _ kne); eauto. destruct d. f_equal. eapply IHdecls. now rewrite kne.
+  f_equal.
+  intros hne.
+  destruct (KernameSet.mem kn deps') eqn:e'.
+  rewrite <- hne in e'. congruence.
+  now eapply IHdecls.
+Qed.
+
+Lemma trans_env_erase_global_decls {X_type X} decls univs retro prf deps deps' ignored :
+  (forall k, ignored k = false) ->
+  KernameSet.Subset deps deps' ->
+  EGlobalEnv.extends (trans_env (@Erasure.erase_global_decls_deps_recursive X_type X decls univs retro prf deps ignored))
+    (filter_deps deps' (trans_env (@Erasure.erase_global_decls_recursive X_type X decls univs retro prf))).
+Proof.
+  induction decls in X_type, X, deps, deps', ignored, prf |- *.
+  - now cbn.
+  - cbn. intros hign hsub.
+    destruct a. destruct g.
+    destruct (KernameSet.mem k deps) eqn:e; cbn [map filter_deps].
+    assert (KernameSet.mem k deps') as ->.
+    { eapply KernameSet.mem_spec in e.
+      now apply KernameSet.mem_spec. }
+    set (er := Erasure.erase_global_decl _ _ _ _ _).
+    set (er' := Erasure.erase_global_decl _ _ _ _ _).
+    set (prf' := fun (Σ : PCUICAst.PCUICEnvironment.global_env) => _).
+    assert (trans_global_decl er = trans_global_decl er'). admit.
+    rewrite <- H.
+    destruct (trans_global_decl er) eqn:eqr.
+    rewrite hign.
+    eapply extends_cons.
+    unfold trans_env in IHdecls.
+    eapply (IHdecls _ _ prf'); eauto. cbn [negb].
+    intros kn.
+    rewrite !KernameSet.union_spec.
+Admitted.
+
+Lemma wf_erase_global_decl :
+  forall (H := EWellformed.all_env_flags)
+        X_type X
+        (k : kername) (g : PCUICAst.PCUICEnvironment.global_decl)
          (decls : list (kername * PCUICAst.PCUICEnvironment.global_decl))
-         (univs : Universes.ContextSet.t) retros w wt (Σex : global_env),
+         (univs : Universes.ContextSet.t) retros prf w wt (Σex : global_env) prf' seeds ignored,
+    let eg := (@Erasure.erase_global_decl X_type
+    (abstract_make_wf_env_ext X (PCUICAst.PCUICLookup.universes_decl_of_decl g) prf)
+    ({| PEnv.universes := univs; PEnv.declarations := decls; PEnv.retroknowledge := retros |},
+      PCUICAst.PCUICLookup.universes_decl_of_decl g)
+    w k g wt) in
+    (forall kn, ignored kn = false) ->
+    Σex = @Erasure.erase_global_decls_deps_recursive X_type X decls univs retros prf'
+      (KernameSet.union (Erasure.decl_deps eg) seeds) ignored ->
     EWellformed.wf_glob (trans_env Σex) ->
     EWellformed.wf_global_decl
       (trans_env Σex)
-      (trans_global_decl
-         (Erasure.erase_global_decl
-            ({| PEnv.universes := univs; PEnv.declarations := decls; PEnv.retroknowledge := retros |},
-              PCUICAst.PCUICLookup.universes_decl_of_decl g)
-            w k g wt)) = true.
+      (trans_global_decl eg) = true.
 Proof.
-  intros H k g decls univs w wt Σex wf_global.
+  intros H X_type X k g decls univs retros prf w wt Σex prf' seeds ignored eg hign eqex wf_global.
+  revert eqex. subst eg.
   unfold Erasure.erase_global_decl.
   destruct g.
   - destruct (Erasure.erase_constant_decl) eqn:Hdecl.
@@ -98,11 +163,33 @@ Proof.
       destruct (Erasure.flag_of_type), conv_ar;try congruence.
       inversion Hdecl;subst;clear Hdecl.
       unfold trans_global_decl,trans_cst.
-      cbn.
+      cbn [EWellformed.wf_global_decl].
       unfold MCOption.option_default.
-      (* global_erased_with_deps *)
-      (* erase_constant_body_correct'' *)
-Qed *)
+      destruct EAst.cst_body eqn:heq.
+      set (deps := KernameSet.union _ _).
+      unshelve eapply (erase_constant_body_correct'' (X_type := X_type) (decls := decls) seeds) in heq as [[t0 [T [[] ?]]]].
+      shelve. intros. eapply Erasure.fake_normalization; tea.
+      { intros. now rewrite (prf' _ H0). }
+      2:exact w.
+      intros ->.
+      eapply EWellformed.extends_wellformed; tea.
+      set (prf'' := fun _ => _). clearbody prf''. cbn in prf''.
+      rewrite erase_global_deps_erase_global.
+      clear.
+      induction decls. red; auto.
+      cbn -[Erasure.erase_global_decls_deps_recursive].
+      destruct a as [kn []].
+      set (prf0 := (fun (pf : _) => _)).
+      set (prf1 := (fun (pf : _) => _)).
+      set (prf2 := (fun (pf : _) => _)).
+      clearbody prf2.
+      cbn -[erase_global Erasure.erase_global_decls_deps_recursive].
+      destruct (KernameSet.mem _ _) eqn:e.
+      set (prf3 := (fun (pf : _) => _)).
+      clearbody prf3.
+
+
+Admitted.
 
 
 Ltac invert_wf :=
@@ -112,17 +199,16 @@ Ltac invert_wf :=
   | [H : P.on_global_decls_data _ _ _ _ _ _ _ |- _] => inversion H; subst; clear H; cbn in *
   end.
 
-(*
-Lemma wf_erase_global_decls_recursive `{EWellformed.EEnvFlags} :
-  forall decls univs retros w seeds (ignored : kername -> bool),
-    let Σex :=
-      Erasure.erase_global_decls_deps_recursive decls univs retros w seeds ignored in
+Lemma wf_erase_global_decls_recursive (H := EWellformed.all_env_flags) :
+  forall X_type X decls univs retros w seeds (ignored : kername -> bool),
+    (forall k, ignored k = false) ->
+    let Σex := @Erasure.erase_global_decls_deps_recursive X_type X decls univs retros w seeds ignored in
     EWellformed.wf_glob (trans_env Σex).
 Proof.
-  intros decls univs retros w seeds ignored ?.
+  intros X_type X decls univs retros w seeds ignored hign ?.
   subst Σex.
   revert seeds.
-  induction decls;intros seeds;auto;try constructor.
+  induction decls in X_type, X, w |- *;intros seeds;auto;try constructor.
   simpl.
   destruct a;simpl.
   destruct (KernameSet.mem _ _);cbn.
@@ -132,21 +218,22 @@ Proof.
       apply IHdecls.
     * cbn.
       remember (KernameSet.union _ _) as kns.
-      clear Heqkns.
+      rewrite hign in Heqkns. cbn in Heqkns.
       remember (Erasure.erase_global_decls_deps_recursive decls univs _ _ _ _) as Σex.
       assert (EWellformed.wf_glob (trans_env Σex)) by now subst Σex.
-      now apply wf_erase_global_decl.
+      rewrite -/(trans_env _).
+      eapply wf_erase_global_decl; eauto. rewrite HeqΣex. f_equal. exact Heqkns.
     * sq.
       apply OptimizePropDiscr.trans_env_fresh_global.
       apply fresh_globals_erase_global_decl_rec.
       change decls with (PEnv.declarations
         {| PEnv.universes := univs; PEnv.declarations := decls; PEnv.retroknowledge := retros |}).
-      apply PCUICWfEnvImpl.wf_fresh_globals.
-      repeat invert_wf;split;auto;split;auto.
+      eapply Erasure.abstract_eq_wf in w as [? []].
+      apply PCUICWfEnvImpl.wf_fresh_globals; eauto.
+      eapply Erasure.wf_pop_decl in X0; trea. eapply X0.
       apply fresh_global_erase_global_decl_rec.
-      change decls with (PEnv.declarations
-        {| PEnv.universes := univs; PEnv.declarations := decls; PEnv.retroknowledge := retros |}).
-      now repeat invert_wf.
+      eapply Erasure.abstract_eq_wf in w as [? []].
+      eapply PCUICWfEnvImpl.wf_fresh_globals in X0. now depelim X0.
   - apply IHdecls.
 Qed.
 
@@ -157,19 +244,25 @@ Lemma optimize_correct `{EWellformed.EEnvFlags} Σ fgΣ t v :
   @Prelim.Ee.eval default_wcbv_flags (trans_env Σ) t v ->
   @Prelim.Ee.eval
       (EWcbvEval.disable_prop_cases opt_wcbv_flags)
-      (trans_env (OptimizePropDiscr.optimize_env Σ fgΣ))
-      (EOptimizePropDiscr.optimize (EEnvMap.GlobalContextMap.make (trans_env Σ) (OptimizePropDiscr.trans_env_fresh_globals _ fgΣ)) t)
-      (EOptimizePropDiscr.optimize (EEnvMap.GlobalContextMap.make (trans_env Σ) (OptimizePropDiscr.trans_env_fresh_globals _ fgΣ)) v).
+      (trans_env (map (on_snd (remove_match_on_box_decl (EEnvMap.GlobalContextMap.make (trans_env Σ) (OptimizePropDiscr.trans_env_fresh_globals _ fgΣ)))) Σ))
+      (EOptimizePropDiscr.remove_match_on_box (EEnvMap.GlobalContextMap.make (trans_env Σ) (OptimizePropDiscr.trans_env_fresh_globals _ fgΣ)) t)
+      (EOptimizePropDiscr.remove_match_on_box (EEnvMap.GlobalContextMap.make (trans_env Σ) (OptimizePropDiscr.trans_env_fresh_globals _ fgΣ)) v).
 Proof.
   intros cl_t cl_env wfg ev.
-  rewrite OptimizePropDiscr.trans_env_optimize_env.
   remember (EEnvMap.GlobalContextMap.make _ _) as Σ0.
-  unshelve eapply (EOptimizePropDiscr.optimize_correct (fl := default_wcbv_flags) (Σ := Σ0));subst;cbn;eauto.
+  assert (trans_env (map (on_snd (remove_match_on_box_decl Σ0)) Σ) =
+    EOptimizePropDiscr.remove_match_on_box_env Σ0) as ->.
+  { cbn. rewrite /trans_env HeqΣ0 map_map_compose. cbn. rewrite /trans_env.
+    rewrite map_map_compose /on_snd. cbn. eapply map_ext.
+    intros [[] []]; cbn. destruct c as [[] []] => //. reflexivity.
+    do 2 f_equal. rewrite /EOptimizePropDiscr.remove_match_on_box_constant_decl /=.
+    now destruct o; cbn. }
+  unshelve eapply (EOptimizePropDiscr.remove_match_on_box_correct (fl := default_wcbv_flags) (Σ := Σ0));subst;cbn;eauto.
 Qed.
 
 
 Theorem extract_correct
-        `{EWellformed.EEnvFlags}
+        (H := EWellformed.all_env_flags)
         (wfl := opt_wcbv_flags)
         (Σ : P.global_env_ext) (wfΣ : ∥wf_ext Σ∥)
         kn ui ind c ui' ignored exΣ :
@@ -188,24 +281,27 @@ Proof.
   destruct dearg_transform eqn:dt; cbn -[dearg_transform] in *; [|congruence].
   injection ex as ->.
   destruct wfΣ.
-  eapply erases_correct with (Σ' := trans_env (Erasure.erase_global_decls_deps_recursive (PCUICAst.PCUICEnvironment.declarations Σ)
-               (PCUICAst.PCUICEnvironment.universes Σ) _ (wf_squash (sq w))
+  eapply erases_correct with
+    (Σ' := trans_env (Erasure.erase_global_decls_deps_recursive (PCUICAst.PCUICEnvironment.declarations Σ)
+               (PCUICAst.PCUICEnvironment.universes Σ) _ _
                (KernameSet.singleton kn) ignored)) in ev as (erv&erase_to&[erev]);eauto.
   + depelim erase_to;[|easy].
     constructor.
     eapply dearg_transform_correct; eauto.
     clear dt.
-    eapply (@OptimizePropDiscr.optimize_correct _ default_wcbv_flags _ _ (tConst kn) (tConstruct ind c []));eauto.
+    eapply (@optimize_correct _ _ _ (tConst kn) (tConstruct ind c []));eauto.
     * remember (Erasure.erase_global_decls_deps_recursive _ _ _ _ _ _) as eΣ.
-      assert (EWellformed.wf_glob (trans_env eΣ)) by now subst eΣ;eapply wf_erase_global_decls_recursive.
+      assert (EWellformed.wf_glob (trans_env eΣ)).
+      { subst eΣ. now eapply wf_erase_global_decls_recursive. }
       now apply EWellformed.wellformed_closed_env.
-    * eapply wf_erase_global_decls_recursive.
+    * eapply wf_erase_global_decls_recursive; auto.
+  + now eexists.
   + eapply inversion_Const in wt as (?&?&?&?&?); auto.
     clear dt.
     eapply global_erased_with_deps_erases_deps_tConst; eauto.
     destruct Σ as [Σ0 univ_decls].
     destruct Σ0 as [univs Σ1].
-    apply wf_ext_wf in w as w1.
+    apply wf_ext_wf in w as w1. cbn.
     eapply erase_global_decls_deps_recursive_correct;eauto.
     * unfold PCUICAst.declared_constant in *.
       cbn.
@@ -213,9 +309,9 @@ Proof.
       intros eq. set (env := {| PEnv.declarations := Σ1 |}) in *.
       eapply (lookup_global_In_wf _ env) in d; eauto.
     * now apply KernameSet.singleton_spec.
+    Unshelve. eapply fresh_globals_erase_global_decl_rec.
+      now eapply PCUICWfEnvImpl.wf_fresh_globals.
 Qed.
-
-*)
 
 (* Print Assumptions extract_correct. *)
 
